James C - more cleanup (and some abbreviations)

isabelle/Chapter10_1_Language.thy
@@ -12,7 +12,7 @@ datatype expr =
   Var var
 | Zero
 | Suc expr
-| Rec expr expr expr
+| Iter expr expr expr
 | Lam type expr
 | Appl expr expr
 | Triv
@@ -20,33 +20,32 @@ datatype expr =
 | ProjL expr
 | ProjR expr
 
-primrec insert :: "var => expr => expr"
-where "insert n (Var v) = Var (incr n v)"
-    | "insert n Zero = Zero"
-    | "insert n (Suc e) = Suc (insert n e)"
-    | "insert n (Rec et e0 es) = Rec (insert n et) (insert n e0) (insert (next (next n)) es)"
-    | "insert n (Lam t e) = Lam t (insert (next n) e)"
-    | "insert n (Appl e1 e2) = Appl (insert n e1) (insert n e2)"
-    | "insert n Triv = Triv"
-    | "insert n (Pair e1 e2) = Pair (insert n e1) (insert n e2)"
-    | "insert n (ProjL e) = ProjL (insert n e)"
-    | "insert n (ProjR e) = ProjR (insert n e)"
+primrec insert :: "var \<Rightarrow> expr \<Rightarrow> expr" where 
+  "insert n (Var v) = Var (incr n v)"
+| "insert n Zero = Zero"
+| "insert n (Suc e) = Suc (insert n e)"
+| "insert n (Iter et e0 es) = Iter (insert n et) (insert n e0) (insert (next n) es)"
+| "insert n (Lam t e) = Lam t (insert (next n) e)"
+| "insert n (Appl e1 e2) = Appl (insert n e1) (insert n e2)"
+| "insert n Triv = Triv"
+| "insert n (Pair e1 e2) = Pair (insert n e1) (insert n e2)"
+| "insert n (ProjL e) = ProjL (insert n e)"
+| "insert n (ProjR e) = ProjR (insert n e)"
 
-primrec subst :: "expr => var => expr => expr"
-where "subst e' n (Var v) = (if v = n then e' else Var (subr n v))"
-    | "subst e' n Zero = Zero"
-    | "subst e' n (Suc e) = Suc (subst e' n e)"
-    | "subst e' n (Rec et e0 es) = 
-                      Rec (subst e' n et) (subst e' n e0) 
-                          (subst (insert first (insert first e')) (next (next n)) es)"
-    | "subst e' n (Lam t e) = Lam t (subst (insert first e') (next n) e)"
-    | "subst e' n (Appl e1 e2) = Appl (subst e' n e1) (subst e' n e2)"
-    | "subst e' n Triv = Triv"
-    | "subst e' n (Pair e1 e2) = Pair (subst e' n e1) (subst e' n e2)"
-    | "subst e' n (ProjL e) = ProjL (subst e' n e)"
-    | "subst e' n (ProjR e) = ProjR (subst e' n e)"
+primrec subst :: "expr \<Rightarrow> var \<Rightarrow> expr \<Rightarrow> expr" where 
+  "subst e' n (Var v) = (if v = n then e' else Var (subr n v))"
+| "subst e' n Zero = Zero"
+| "subst e' n (Suc e) = Suc (subst e' n e)"
+| "subst e' n (Iter et e0 es) = 
+    Iter (subst e' n et) (subst e' n e0) (subst (insert first e') (next n) es)"
+| "subst e' n (Lam t e) = Lam t (subst (insert first e') (next n) e)"
+| "subst e' n (Appl e1 e2) = Appl (subst e' n e1) (subst e' n e2)"
+| "subst e' n Triv = Triv"
+| "subst e' n (Pair e1 e2) = Pair (subst e' n e1) (subst e' n e2)"
+| "subst e' n (ProjL e) = ProjL (subst e' n e)"
+| "subst e' n (ProjR e) = ProjR (subst e' n e)"
 
-lemma [simp]: "canswap m n ==> insert m (insert n e) = insert (next n) (insert m e)"
-by (induction e arbitrary: n m, simp_all)
+lemma [simp]: "canswap m n \<Longrightarrow> insert m (insert n e) = insert (next n) (insert m e)"
+  by (induction e arbitrary: n m) simp_all
 
 end
