isabelle/Chapter11_4_Abbreviations.thy
@@ -1,0 +1,101 @@
+theory Chapter11_4_Abbreviations
+imports Chapter11_3_Evaluation
+begin
+
+(* booleans *)
+
+abbreviation Bool :: type where
+  "Bool \<equiv> Sum Unit Unit"
+
+abbreviation Tru :: expr where
+  "Tru \<equiv> InL Unit Unit Triv"
+
+abbreviation Fls :: expr where
+  "Fls \<equiv> InR Unit Unit Triv"
+
+abbreviation If :: "expr \<Rightarrow> expr \<Rightarrow> expr \<Rightarrow> expr" where
+  "If e et ef \<equiv> Case e (insert first et) (insert first ef)"
+
+lemma tc_true: "typecheck gam Tru Bool"
+  by simp
+
+lemma tc_fals: "typecheck gam Fls Bool"
+  by simp
+
+lemma tc_if: "typecheck gam e Bool \<Longrightarrow> typecheck gam et t \<Longrightarrow> typecheck gam ef t \<Longrightarrow> 
+    typecheck gam (If e et ef) t"
+  by simp
+
+lemma [simp]: "is_val Tru"
+  by simp
+
+lemma [simp]: "is_val Fls"
+  by simp
+
+lemma [simp]: "\<not> is_val (If e et ef)"
+  by simp
+
+lemma eval_if_1: "eval e e' \<Longrightarrow> eval (If e et ef) (If e' et ef)"
+  by simp
+
+lemma eval_if_2: "eval (If Tru et ef) et"
+  proof -
+    from eval_case_2 is_val.simps(7) have "eval (Case (InL Unit Unit Triv) (insert first et) 
+      (insert first ef)) (subst Triv first (insert first et))" by blast
+    thus "eval (If Tru et ef) et" by simp
+  qed
+
+lemma eval_if_3: "eval (If Fls et ef) ef"
+  proof -
+    from eval_case_3 is_val.simps(7) have "eval (Case (InR Unit Unit Triv) (insert first et) 
+      (insert first ef)) (subst Triv first (insert first ef))" by blast
+    thus "eval (If Fls et ef) ef" by simp
+  qed
+
+(* options *)
+
+abbreviation Option :: "type \<Rightarrow> type" where
+  "Option \<equiv> Sum Unit"
+
+abbreviation Null :: "type \<Rightarrow> expr" where
+  "Null t \<equiv> InL Unit t Triv"
+
+abbreviation Just :: "type \<Rightarrow> expr \<Rightarrow> expr" where
+  "Just t e \<equiv> InR Unit t e"
+
+abbreviation Which :: "expr \<Rightarrow> expr \<Rightarrow> expr \<Rightarrow> expr" where
+  "Which e e0 ej \<equiv> Case e (insert first e0) ej"
+
+lemma tc_null: "typecheck gam (Null t) (Option t)"
+  by simp
+
+lemma tc_just: "typecheck gam e t \<Longrightarrow> typecheck gam (Just t e) (Option t)"
+  by simp
+
+lemma tc_which: "typecheck gam e (Option t) \<Longrightarrow> typecheck gam e0 tt \<Longrightarrow> 
+    typecheck (extend gam t) ej tt \<Longrightarrow> typecheck gam (Which e e0 ej) tt"
+  by simp
+
+lemma [simp]: "is_val (Null t)"
+  by simp
+
+lemma [simp]: "is_val (Just t e) = is_val e"
+  by simp
+
+lemma [simp]: "\<not> is_val (Which e e0 ej)"
+  by simp
+
+lemma eval_which_1: "eval e e' \<Longrightarrow> eval (Which e e0 ej) (Which e' e0 ej)"
+  by simp
+
+lemma eval_which_2: "eval (Which (Null t) e0 ej) e0"
+  proof -
+    from eval_case_2 is_val.simps(7) have "eval (Case (InL Unit t Triv) (insert first e0) ej) 
+      (subst Triv first (insert first e0))" by blast
+    thus "eval (Which (Null t) e0 ej) e0" by simp
+  qed
+
+lemma eval_which_3: "is_val e \<Longrightarrow> eval (Which (Just t e) e0 ej) (subst e first ej)"
+  by simp
+
+end
